We succeeded in describing parallel quantum programs using axiom interfaces. We defined the operational semantics and verified all the claimed properties. It is compositional!

Ranko/Parallel/para.v
@@ -1,6 +1,8 @@
 From Ranko Require Import TerminalDogma.premises.
 From Coq Require Import Classical.
-
+From Coq Require Import PropExtensionality.
+From Coq Require Import FunctionalExtensionality.
+From Coq Require Import Arith.
 
 Set Implicit Arguments.
 Unset Strict Implicit.
@@ -36,6 +38,9 @@ Axiom PDenSet : Hspace -> Type.
 (** The universal set of this partial density operator *)
 Axiom PDenSet_uni : forall {H}, PDenSet H.
 
+(** Here we have the difference : we need to perform 'union' on the program
+    state, but we cannot union two density operators. Therefore density 
+    operator sets are needed.*)
 Axiom PDenSet_Union : forall {H : Hspace}, PDenSet H -> PDenSet H -> PDenSet H.
 Axiom PDenSet_Add : forall {H : Hspace}, PDenSet H -> PDenSet H -> PDenSet H.
 Notation " A '∪' B " := (@PDenSet_Union _ A B) (at level 10).
@@ -204,13 +209,13 @@ Definition Step {qs : QvarScope} (S1 S2: prog qs)
     end.
 
 (** Define the operational semantics *)
-Fixpoint OpSem {qs : QvarScope} (c : cfg qs) (n : nat) : PDenSet qs :=
+Fixpoint OpSemN {qs : QvarScope} (c : cfg qs) (n : nat) : PDenSet qs :=
     match c with
     | <{ ↓ , rho_s }> => rho_s
     | <{ P , rho_s }> => 
         match n with
-        | O => PDenSet_uni
-        | S n' => 
+        | 0 => PDenSet_uni
+        | n'.+1 => 
             match P with
             | Skip => 
                 rho_s
@@ -221,59 +226,76 @@ Fixpoint OpSem {qs : QvarScope} (c : cfg qs) (n : nat) : PDenSet qs :=
             | qv *= U => 
                 Uapply U rho_s
             | If m [[ qv_m ]] Then P0 Else P1 End =>
-                (OpSem <{ P0, Mapply m rho_s true }> n')
-                + (OpSem <{ P1, Mapply m rho_s false }> n')
+                (OpSemN <{ P0, Mapply m rho_s true }> n')
+                + (OpSemN <{ P1, Mapply m rho_s false }> n')
             | While m [[ qv_m ]] Do P0 End  =>
-                (OpSem <{ P0;; While m [[ qv_m ]] Do P0 End 
+                (OpSemN <{ P0;; While m [[ qv_m ]] Do P0 End 
                         , Mapply m rho_s true }> n')
                 + Mapply m rho_s false
             | S1 ;; S2 => 
-                OpSem <{ S2 , OpSem <{S1, rho_s}> n' }> n'
+                OpSemN <{ S2 , OpSemN <{S1, rho_s}> n' }> n'
             | << P >> => 
-                OpSem <{ P, rho_s }> n'
+                OpSemN <{ P, rho_s }> n'
             | [ S1 // S2 ] => 
                 (** Note that here we give a different interpretation of 
                     nested parallel composition *)
-                (OpSem <{ Step S1 S2 true , rho_s }> n')
-                ∪ (OpSem <{ Step S1 S2 false , rho_s }> n')
+                (OpSemN <{ Step S1 S2 true , rho_s }> n')
+                ∪ (OpSemN <{ Step S1 S2 false , rho_s }> n')
             end
         end
     end.
 
 
-Lemma OpSem_seq_ex {qs : QvarScope} S0 S1 :
-        forall rho_s n, exists a b, OpSem <{ S0 ;; S1, rho_s }> n = 
-                @OpSem qs <{ S1 , OpSem <{ S0, rho_s}> a }> b.
+Lemma OpSemN_seq_ex {qs : QvarScope} S0 S1 :
+        forall rho_s n, exists a b, OpSemN <{ S0 ;; S1, rho_s }> n = 
+                @OpSemN qs <{ S1 , OpSemN <{ S0, rho_s}> a }> b.
 Proof.
     (** This property does not hold in the finite situation, because S0 can
         have branches of different lengths. *)
 Abort.
-    
 
-
-Lemma OpSem_if {qs : QvarScope} qv_m m S0 S1: 
-        forall rho_s n, OpSem <{ If m [[ qv_m ]] Then S0 Else S1 End , rho_s }> n.+1
-                    = OpSem <{ S0, Mapply m rho_s true }> n
-                        + @OpSem qs <{ S1, Mapply m rho_s false }> n.
+Lemma OpSemN_seq {qs : QvarScope} S0 S1 :
+        forall rho_s n, OpSemN <{ S0 ;; S1, rho_s }> n.+1 = 
+                @OpSemN qs <{ S1 , OpSemN <{ S0, rho_s}> n }> n.
 Proof. move => rho_s. by case. Qed.
 
-Lemma OpSem_while {qs : QvarScope} qv_m m S0:
-        forall rho_s n, OpSem <{ While m [[ qv_m ]] Do S0 End , rho_s }> n.+1
-                    = OpSem <{ S0;; While m [[ qv_m ]] Do S0 End , 
+
+Lemma OpSemN_if {qs : QvarScope} qv_m m S0 S1: 
+        forall rho_s n, OpSemN <{ If m [[ qv_m ]] Then S0 Else S1 End , rho_s }> n.+1
+                    = OpSemN <{ S0, Mapply m rho_s true }> n
+                        + @OpSemN qs <{ S1, Mapply m rho_s false }> n.
+Proof. move => rho_s. by case. Qed.
+
+Lemma OpSemN_while {qs : QvarScope} qv_m m S0:
+        forall rho_s n, OpSemN <{ While m [[ qv_m ]] Do S0 End , rho_s }> n.+1
+                    = OpSemN <{ S0;; While m [[ qv_m ]] Do S0 End , 
                             Mapply m rho_s true }> n
                         + (@Mapply qs qv_m m rho_s false).
 Proof. move => rho_s. by case. Qed.
+
+Lemma OpSemN_atom {qs : QvarScope} P :
+        forall rho_s n, OpSemN <{ <<P>>, rho_s }> n.+1
+                    = @OpSemN qs <{ P, rho_s }> n.
+Proof. move => rho_s. by case. Qed.
+
+Lemma OpSemN_parallel {qs : QvarScope} S1 S2 :
+        forall rho_s n, OpSemN <{ [ S1 // S2 ], rho_s }> n.+1
+                    = (OpSemN <{ Step S1 S2 true , rho_s }> n)
+                        ∪ (@OpSemN qs <{ Step S1 S2 false , rho_s }> n).
+Proof. move => rho_s. by case. Qed.
+
 
 (** Arguments about order *)
 Axiom PDenSetOrder : forall {H : Hspace}, PDenSet H -> PDenSet H -> Prop.
 Notation " A '⊑' B " := (PDenSetOrder A B) (at level 60).
 
-Locate reflexive.
 
 Axiom PDenSetOrder_refl : 
     forall H, Relation_Definitions.reflexive _ (@PDenSetOrder H).
 Axiom PDenSetOrder_trans : 
     forall H, Relation_Definitions.transitive _ (@PDenSetOrder H).
+Axiom PDenSetOrder_asymm :
+    forall H, Relation_Definitions.antisymmetric _ (@PDenSetOrder H).
 
 Add Parametric Relation H : _ (@PDenSetOrder H)
     reflexivity proved by (@PDenSetOrder_refl H)
@@ -288,7 +310,23 @@ Add Parametric Morphism {H : Hspace} : (@PDenSet_Add H)
 Proof.
 Admitted.
 
-Check InitStt.
+Lemma PDenSetOrder_add_split {H : Hspace} :
+    forall {rho_s1 rho_s2 rho_s1' rho_s2': PDenSet H}, 
+        rho_s1 ⊑ rho_s1' -> rho_s2 ⊑ rho_s2' 
+            -> rho_s1 + rho_s2 ⊑ rho_s1' + rho_s2'.
+Proof. move => a b c d Hac Hbd. rewrite Hac Hbd. by reflexivity. Qed.
+
+Add Parametric Morphism {H : Hspace} : (@PDenSet_Union H)
+    with signature (@PDenSetOrder H) ==> (@PDenSetOrder H) 
+                    ==> (@PDenSetOrder H) as union_mor_le.
+Proof.
+Admitted.
+
+Lemma PDenSetOrder_union_split {H : Hspace} :
+    forall {rho_s1 rho_s2 rho_s1' rho_s2': PDenSet H}, 
+        rho_s1 ⊑ rho_s1' -> rho_s2 ⊑ rho_s2' 
+            -> rho_s1 ∪ rho_s2 ⊑ rho_s1' ∪ rho_s2'.
+Proof. move => a b c d Hac Hbd. rewrite Hac Hbd. by reflexivity. Qed.
 
 Axiom PDenSetOrder_Init : 
     forall {qs : QvarScope} r1 r2 (qv : qs), r1 ⊑ r2 -> InitStt qv r1 ⊑ InitStt qv r2.
@@ -299,95 +337,539 @@ Axiom PDenSetOrder_M :
     forall {qs : QvarScope} r1 r2 (qv_m : qs) (m : MeaOpt qv_m) (result : bool),
         r1 ⊑ r2 -> Mapply m r1 result ⊑ Mapply m r2 result.
 
-Lemma PDenSetOrder_add_split {H : Hspace} :
-    forall {rho_s1 rho_s2 rho_s1' rho_s2': PDenSet H}, 
-        rho_s1 ⊑ rho_s1' -> rho_s2 ⊑ rho_s2' 
-            -> rho_s1 + rho_s2 ⊑ rho_s1' + rho_s2'.
-Proof. move => a b c d Hac Hbd. rewrite Hac Hbd. by reflexivity. Qed.
 
-(* 用这个引理证递增的结论 *)
-Lemma PDenSetOrder_OpSem_strong {qs : QvarScope} :
-    forall (S0 : prog qs) (r1 r2 : PDenSet qs) n n0, 
-        n0 <= n -> r1 ⊑ r2 -> OpSem <{ S0 , r1 }> n0 ⊑ OpSem <{ S0 , r2 }> n0.
-Proof.
-
-    move => S0 r1 r2 n n0 Hn0 Hr1r2.
-    case : n0 Hn0. move =>_. by apply PDenSet_uni_least.
-    (*
-    elim : S0 r1 r2 Hr1r2.
-    (* skip *)
-    by move => r1 r2 Hr1r2 n0 Hn0 => /=.
-    (* abort *)
-    move => r1 r2 Hr1r2 n0 Hn0 => /=. by reflexivity.
-    (* init *)
-    move => qv r1 r2 Hr1r2 n0 => //=. by apply PDenSetOrder_Init.
-    (* unitary *)
-    move => qv r1 r2 Hr1r2 U n => //=. by apply PDenSetOrder_U.
-    (* sequential composition first *)
-    3: apply SeqLemma.
-    (* if *)
-    move => qv_m m S0 IHS0 S1 IHS1 r1 r2 Hr1r2 n //=.
-    case: n. by reflexivity.
-    move => n. apply PDenSetOrder_add_split. 
-    apply IHS0. by apply PDenSetOrder_M.
-    apply IHS1. by apply PDenSetOrder_M.
-    (* while *)
-    move => qv_m m S0 IHS0 r1 r2 Hr1r2 n.
-    elim: n r1 r2 Hr1r2. move => r1 r2 Hr1r2 //=. by rewrite !PDenSet_Add_uni_l; reflexivity.
-    move => n IHn r1 r2 Hr1r2. apply PDenSetOrder_add_split; last first. by apply PDenSetOrder_M.
-    apply SeqLemma. apply IHS0.
-    *)
-Admitted.
-
-Lemma PDenSetOrder_OpSem {qs : QvarScope} :
-    forall (S0 : prog qs) (r1 r2 : PDenSet qs) n, 
-        r1 ⊑ r2 -> OpSem <{ S0 , r1 }> n ⊑ OpSem <{ S0 , r2 }> n.
-Proof.
+(* The relation between OpSemN and order *)
+Lemma PDenSetOrder_OpSemN_strong {qs : QvarScope} :
+    forall (S0 : prog qs) (r1 r2 : PDenSet qs) n i, 
+        i <= n -> r1 ⊑ r2 -> OpSemN <{ S0 , r1 }> i ⊑ OpSemN <{ S0 , r2 }> i.
+Proof. 
     move => S0 r1 r2 n.
-    by apply (@PDenSetOrder_OpSem_strong qs S0 r1 r2 n n).
+
+    (* induction on n *)
+    elim: n S0 r1 r2.
+    (* induction basis, n = 0*)
+    move => S0 r1 r2 i. rewrite leqn0 => /eqP ->. by reflexivity.
+
+    (* induction step, process i=0 first *)
+    move => n IHn S0 r1 r2 i Hi Hr1r2. case: i Hi.
+    by reflexivity.
+
+    move => i Hi.
+    (* case on programs *)
+    case: S0.
+    (* skip *)
+    by move => //=.
+    (* abort *)
+    move => //=. by reflexivity.
+    (* init *)
+    move => qv //=. by apply PDenSetOrder_Init.
+    (* unitary *)
+    move => qv U //=. by apply PDenSetOrder_U.
+    (* if *)
+    move => qv_m m S0 S1 //=. 
+    by apply PDenSetOrder_add_split; apply /IHn => //; apply PDenSetOrder_M.
+    (* while *)
+    move => qv_m m S0 //=.
+    apply PDenSetOrder_add_split; last first. by apply PDenSetOrder_M.
+    apply IHn => //. by apply PDenSetOrder_M.
+    (* sequence *)
+    move => S1 S2 //=. apply IHn => //. by apply IHn => //.
+    (* atom *)
+    move => S0 => //=. by apply IHn => //.
+    (* parallel *)
+    move => S1 S2. rewrite !OpSemN_parallel. 
+    by apply PDenSetOrder_union_split; apply IHn.
 Qed.
 
-Lemma OpSem_inc {qs : QvarScope} : 
-    forall (c : cfg qs) n, OpSem c n ⊑ OpSem c n.+1.
+Lemma PDenSetOrder_OpSemN {qs : QvarScope} :
+    forall (S0 : prog qs) (r1 r2 : PDenSet qs) n, 
+        r1 ⊑ r2 -> OpSemN <{ S0 , r1 }> n ⊑ OpSemN <{ S0 , r2 }> n.
+Proof.
+    move => S0 r1 r2 n.
+    by apply (@PDenSetOrder_OpSemN_strong qs S0 r1 r2 n n).
+Qed.
+
+
+
+(** Prove that [OpSemN c i] is increasing when i increases. *)
+Lemma OpSemN_inc_strong {qs : QvarScope} : 
+    forall (c : cfg qs) n i, i <= n -> OpSemN c i ⊑ OpSemN c i.+1.
 Proof.
     (** process terminated configurations first *)
     move => []; last first.
-    move => rho_s. case => //=; by reflexivity.
+    move => rho_s n. case => //=; by reflexivity.
 
-    (* induction on program *)
-    elim.
+    (* induction on n *)
+    move => S0 rho_s n. elim : n S0 rho_s.
 
-    (* skip, abort *)
-    1, 2 : by move => rho_s /=; case => //=; [ apply PDenSet_uni_least | reflexivity].
-    (* init *)
-    move => qv rho_s /=. by case => //=; [ apply PDenSet_uni_least | reflexivity].
-    (* unitary *)
-    move => qv U rho_s /=. by case => //=; [ apply PDenSet_uni_least | reflexivity].
+    (* induction basi, n = 0 *)
+    move => S0 rho_s i. rewrite leqn0 => /eqP ->. by apply PDenSet_uni_least.
 
-    (* seq first *)
-    3: { move => S1 IHS1 S2 IHS2 rho_s n.
-    case: n. by reflexivity.
-    move => n. elim S1. 
+    (* induction step, process i=0 first *)
+    move => n IHn S0 rho_s. case.
+    move => _ //=. by apply PDenSet_uni_least.
+    
+    (* case on programs *)
+    case : S0 rho_s.
 
-
-    }
-
+    (* skip, abort, init, unitary *)
+    1,2,3,4: move => i Hi => //=; by reflexivity.
+    
     (* if *)
-    move => qv_m m S0 IHS0 S1 IHS1 rho_s. case.
-    by apply PDenSet_uni_least.
-    move => n. rewrite !OpSem_if. 
-    apply PDenSetOrder_add_split. by apply IHS0. by apply IHS1.
+    move => qv_m m S0 S1 rho_s i Hi. rewrite !OpSemN_if.
+    by apply PDenSetOrder_add_split; apply /IHn.
 
     (* while *)
-    move => qv_m m S0 IHS0 rho_s n. move : rho_s. elim: n.
-    by move => rho_s; apply PDenSet_uni_least.
-    move => n IH rho_s. rewrite !OpSem_while.
-    apply PDenSetOrder_add_split; last first. by reflexivity.
-    { case n. by reflexivity. 
-         } 
+    move => qv_m m S0 rho_s i Hi. rewrite !OpSemN_while.
+    apply PDenSetOrder_add_split. by apply /IHn. by reflexivity.
+
+    (* seq *)
+    move => S1 S2 rho_s i Hi. rewrite !OpSemN_seq.
+    transitivity (OpSemN <{ S2, OpSemN <{ S1, rho_s }> i.+1 }> i).
+    apply PDenSetOrder_OpSemN. (* Here the relation on order and OpSemN is used. *)
+    by apply IHn.
+    by apply IHn.
+
+    (* atom *)
+    move => S0 rho_s i Hi. rewrite !OpSemN_atom.
+    by apply IHn.
+
+    (* parallel *)
+    move => S1 S2 rho_s i Hi. rewrite !OpSemN_parallel.
+    apply PDenSetOrder_union_split; by apply IHn.
+Qed.
+
+Lemma OpSemN_inc_step {qs : QvarScope} : 
+    forall (c : cfg qs) n, OpSemN c n ⊑ OpSemN c n.+1.
+Proof. move => c n. by apply (@OpSemN_inc_strong qs c n n). Qed.
+
+Lemma OpSemN_inc {qs : QvarScope} : 
+    forall (c : cfg qs) i n, i <= n -> OpSemN c i ⊑ OpSemN c n.
+Proof.
+    (** process terminated configurations first *)
+    case; last first.
+    move => rho_s. case. case.
+    move => _. by reflexivity.
+    move => n _. by reflexivity.
+    move => i n. elim: n.
+    move => _. by reflexivity.
+    move => n _ _. by reflexivity.
+
+    move => S0 rho_s.
+
+    (* we prove a equivalent proposition, which is easier to be proved. *)
+    have temp : forall (i x : nat),
+        OpSemN <{ S0, rho_s }> i ⊑ OpSemN <{ S0, rho_s }> (x + i)%nat.
+    { move => i. elim. by reflexivity.
+        move => n IHn. replace (n.+1 + i)%nat with (n + i).+1; last first.
+            by [].
+            transitivity (OpSemN <{ S0, rho_s }> (n + i)).
+            by apply IHn.
+            by apply OpSemN_inc_step. }
+
+    move => i n Hi.
+    replace n with (i + (n - i)%nat)%nat; last first.
+    by apply subnKC.
+    
+    replace (i + (n - i))%nat with ((n-i)%nat+i)%nat; last first.
+    apply Nat.add_comm.
+    apply temp.
+Qed.
+
+
+
+
+
+
+(** Define the increasing set and least upper bound *)
+Record chain (H : Hspace) := mk_chain {
+    chain_obj : nat -> PDenSet H;
+    chain_prop : forall n, chain_obj n ⊑ chain_obj n.+1;
+}.
+Notation " ch _[ n ] " := (chain_obj ch n) (at level 40).
+
+(** Convert a singal element into a list *)
+Definition singleton_chain_obj {H : Hspace} rho_s : nat -> PDenSet H :=
+    fun => rho_s.
+
+Lemma singleton_chain_prop {H : Hspace} (rho_s : PDenSet H) 
+    : forall n, singleton_chain_obj rho_s n ⊑ singleton_chain_obj rho_s n.+1.
+Proof. rewrite /singleton_chain_obj => n => //=. by reflexivity. Qed.
+
+Definition singleton_chain {H : Hspace} rho_s : chain H :=
+    mk_chain (singleton_chain_prop rho_s).
+
+Coercion singleton_chain : PDenSet >-> chain.
+
+(** Prove the loose criterion of chain equivalence *)
+Lemma chain_eqP H : forall (ch1 ch2 : chain H),
+        ch1 = ch2 <-> chain_obj ch1 = chain_obj ch2.
+Proof. split. by move => -> //.
+    move => Heq. destruct ch1 as [obj1 p1], ch2 as [obj2 p2]. simpl in Heq.
+    move : p1 p2. rewrite Heq => p1 p2. by rewrite (proof_irrelevance _ p1 p2).
+Qed.
+
+Axiom chain_limit : forall H (ch : chain H), PDenSet H.
+Notation " 'lim→∞' ( ch ) " := (@chain_limit _ ch) (at level 200).
+Axiom chain_limit_ub : forall H (ch : chain H) n,
+    ch _[n] ⊑ lim→∞ (ch).
+Axiom chain_limit_lub : forall H (ch : chain H) rho_ub,
+    (forall n, ch _[n] ⊑ rho_ub) -> lim→∞ (ch) ⊑ rho_ub.
+
+Lemma singleton_chain_limit (H : Hspace) (rho_s : PDenSet H) :
+    lim→∞ (rho_s) = rho_s.
+Proof.
+    apply PDenSetOrder_asymm.
+    apply chain_limit_lub. 
+    rewrite /singleton_chain /singleton_chain_obj => n => //=. by reflexivity.
+    have temp := chain_limit_ub rho_s. by apply (temp 0).
+Qed.
+
+(** Define the operationa semantics (infinite step) *)
+Definition chain_OpSemN {qs : QvarScope} (P : prog qs) rho_s : chain qs :=
+    {|  chain_obj := fun n=>OpSemN <{P,rho_s}> n; 
+        chain_prop := fun n=>OpSemN_inc_step <{P,rho_s}> n |}.
+Lemma chain_OpSemN_n {qs : QvarScope} (P : prog qs) rho_s n :
+        chain_OpSemN P rho_s _[n] = OpSemN <{P, rho_s}> n.
+Proof. by []. Qed.
+    
+Definition OpSem {qs : QvarScope} (P : prog qs) rho_s : PDenSet qs :=
+    lim→∞ (chain_OpSemN P rho_s).
+
+Notation " '⟦' P '⟧' ( rho_s ) " := (@OpSem _ P rho_s).
+
+Lemma OpSem_ub : forall {qs : QvarScope} n (P : prog qs) rho_s, 
+    OpSemN <{P, rho_s}> n ⊑ ⟦ P ⟧ (rho_s).
+Proof. 
+    rewrite /OpSem => qs n P rho_s. rewrite -chain_OpSemN_n. 
+    by apply chain_limit_ub.
+Qed.
+Arguments OpSem_ub {qs} n P rho_s.
+
+Lemma OpSem_lub : forall {qs : QvarScope} (P : prog qs) rho_s rho_ub, 
+    (forall n, OpSemN <{P, rho_s}> n ⊑ rho_ub) -> ⟦ P ⟧ (rho_s) ⊑ rho_ub.
+Proof.
+    rewrite /OpSem => qs P rho_s rho_ub H. apply chain_limit_lub. by apply H.
+Qed.
+
+Lemma OpSem_lubP : forall {qs : QvarScope} (P : prog qs) rho_s rho_ub, 
+    (forall n, OpSemN <{P, rho_s}> n ⊑ rho_ub) <-> ⟦ P ⟧ (rho_s) ⊑ rho_ub.
+Proof. split. by apply OpSem_lub.
+    move => HP n. transitivity (⟦ P ⟧ (rho_s)) => //. 
+    by apply OpSem_ub.
+Qed.
+
+
+(** Properties of Operationl Semantics *)
+
+Lemma OpSem_skip {qs : QvarScope} (rho_s : PDenSet qs):
+    ⟦ Skip ⟧ (rho_s) = rho_s.
+Proof.
+    apply PDenSetOrder_asymm.
+    apply OpSem_lub. case. by apply PDenSet_uni_least.
+    move => n //=. by reflexivity.
+    transitivity (OpSemN <{ Skip, rho_s }> 1). by reflexivity.
+    by apply OpSem_ub.
+Qed.
+
+Lemma OpSem_abort {qs : QvarScope} (rho_s : PDenSet qs):
+    ⟦ Abort ⟧ (rho_s) = PDenSet_uni.
+Proof.
+    apply PDenSetOrder_asymm.
+    apply OpSem_lub. case. by apply PDenSet_uni_least.
+    move => n //=. by reflexivity.
+    transitivity (OpSemN <{ Abort, rho_s }> 1). by reflexivity.
+    by apply OpSem_ub.
+Qed.
+
+Lemma OpSem_init {qs : QvarScope} qv (rho_s : PDenSet qs):
+    ⟦ qv <- 0 ⟧ (rho_s) = InitStt qv rho_s.
+Proof.
+    apply PDenSetOrder_asymm.
+    apply OpSem_lub. case. by apply PDenSet_uni_least.
+    move => n //=. by reflexivity.
+    transitivity (OpSemN <{ qv <- 0, rho_s }> 1). by reflexivity.
+    by apply OpSem_ub.
+Qed.
+
+Lemma OpSem_unitary {qs : QvarScope} qv U (rho_s : PDenSet qs):
+    ⟦ qv *= U ⟧ (rho_s) = Uapply U rho_s.
+Proof.
+    apply PDenSetOrder_asymm.
+    apply OpSem_lub. case. by apply PDenSet_uni_least.
+    move => n //=. by reflexivity.
+    transitivity (OpSemN <{ qv *= U, rho_s }> 1). by reflexivity.
+    by apply OpSem_ub.
+Qed.
+
+(* chain_add *)
+Definition chain_add_obj (H : Hspace) (ch_obj1 ch_obj2 : nat -> PDenSet H) :=
+    fun n => ch_obj1 n + ch_obj2 n.
+Lemma chain_add_obj_prop (H : Hspace) (ch1 ch2 : chain H) :
+    let ch := chain_add_obj (chain_obj ch1) (chain_obj ch2) in 
+        forall n, ch n ⊑ ch n.+1.
+Proof. move => ch n. rewrite /ch /chain_add_obj. apply PDenSetOrder_add_split.
+    by apply ch1. by apply ch2.
+Qed.
+
+(** Add chain is needed for proving if statement *)
+Definition chain_add H (ch1 ch2 : chain H) : chain H :=
+    mk_chain (chain_add_obj_prop ch1 ch2).
+
+(** We still need the assumption that addition is continuous *)
+Axiom add_continuous : forall H (ch1 ch2 : chain H),
+    (lim→∞(ch1)) + (lim→∞(ch2)) = lim→∞ (chain_add ch1 ch2).
+
+
+(* chain_union *)
+Definition chain_union_obj (H : Hspace) (ch1 ch2 : chain H) :=
+    fun n => (ch1 _[n]) ∪ (ch2 _[n]).
+Lemma chain_union_prop (H : Hspace) (ch1 ch2 : chain H) :
+    forall n, chain_union_obj ch1 ch2 n ⊑ chain_union_obj ch1 ch2 n.+1.
+Proof. move => n. rewrite /chain_union_obj. apply PDenSetOrder_union_split.
+    by apply ch1. by apply ch2.
+Qed.
+
+(** Add chain is needed for proving if statement *)
+Definition chain_union H (ch1 ch2 : chain H) : chain H :=
+    mk_chain (chain_union_prop ch1 ch2).
+
+(** We still need the assumption that addition is continuous *)
+Axiom union_continuous : forall H (ch1 ch2 : chain H),
+    (lim→∞(ch1)) ∪ (lim→∞(ch2)) = lim→∞ (chain_union ch1 ch2).
+
+
+Lemma OpSem_if {qs : QvarScope} qv_m m S0 S1 (rho_s : PDenSet qs):
+    ⟦ If m [[qv_m]] Then S0 Else S1 End ⟧ (rho_s) 
+        = ⟦ S0 ⟧ (Mapply m rho_s true) + ⟦ S1 ⟧ (Mapply m rho_s false).
+Proof.
+    apply PDenSetOrder_asymm.
+
+    (*
+           ⟦S0⟧  ⟦S1⟧ ⟦IF⟧
+            0  +  0   0
+                    \
+            1  +  1   1
+                    \
+            2  +  2   2
+                    \
+              ...    ...
+
+    *)
+    (* proof : ⟦S0⟧ + ⟦S1⟧ is the upper bound, therefore larger than lub ⟦IF⟧. *)
+    apply OpSem_lub. case. by apply PDenSet_uni_least.
+    move => n //=. apply PDenSetOrder_add_split; apply OpSem_ub.
+
+    (* proof : ⟦IF⟧ is the upper bound, therefore larger than lub ⟦S0⟧ + ⟦S1⟧.
+        For this purpose we need the continuity of add. *)
+    rewrite ![⟦ _ ⟧ (Mapply m rho_s _)]/OpSem. rewrite add_continuous.
+    apply chain_limit_lub => l. rewrite /chain_add /chain_add_obj => //=.
+    rewrite -OpSemN_if. by apply OpSem_ub.
+Qed.
+
+
+Lemma OpSem_while {qs : QvarScope} qv_m m S0 (rho_s : PDenSet qs):
+    ⟦ While m [[qv_m]] Do S0 End ⟧ (rho_s) 
+        = ⟦ S0 ;; While m [[qv_m]] Do S0 End ⟧ (Mapply m rho_s true) 
+            + Mapply m rho_s false.
+Proof.
+    apply PDenSetOrder_asymm.
+
+    apply OpSem_lub. case. by apply PDenSet_uni_least.
+    move => n //=. apply PDenSetOrder_add_split. 
+    by apply OpSem_ub. by reflexivity.
+
+
+    rewrite [⟦ _ ⟧ (Mapply m rho_s _)]/OpSem.
+
+    (* We need to transform the [Mapply m rho_s false] term into a singleton
+        chain. *)
+    rewrite -(singleton_chain_limit (Mapply m rho_s false)).
+    rewrite add_continuous.
+    apply chain_limit_lub => l. rewrite /chain_add /chain_add_obj => //=.
+    rewrite -OpSemN_while. by apply OpSem_ub.
+Qed.
+
+(* The chain of InitStt ch *)
+Definition InitStt_chain_obj {qs : QvarScope} (qv : qs) (ch : chain qs) :=
+    fun i => InitStt qv (ch _[i]).
+Lemma InitStt_chain_prop {qs : QvarScope} (qv : qs) (ch : chain qs)
+    : forall i, InitStt_chain_obj qv ch i ⊑ InitStt_chain_obj qv ch i.+1.
+Proof.
+    rewrite /InitStt_chain_obj => i. apply PDenSetOrder_Init. by apply ch.
+Qed.
+
+Definition InitStt_chain {qs : QvarScope} (qv : qs) (ch : chain qs) :=
+    mk_chain (InitStt_chain_prop qv ch).
+
+(** We still need the assumption that addition is continuous *)
+Axiom init_continuous : forall {qs : QvarScope} (qv : qs) (ch : chain qs),
+    InitStt qv (lim→∞ (ch)) = lim→∞ (InitStt_chain qv ch).
+
+(* The chain of Uapply U ch *)
+Definition Uapply_chain_obj 
+    {qs : QvarScope} (qv : qs) (U : UnitaryOpt qv) (ch : chain qs) :=
+    fun i => Uapply U (ch _[i]).
+Lemma Uapply_chain_prop 
+    {qs : QvarScope} (qv : qs) (U : UnitaryOpt qv) (ch : chain qs)
+    : forall i, Uapply_chain_obj U ch i ⊑ Uapply_chain_obj U ch i.+1.
+Proof.
+    rewrite /Uapply_chain_obj => i. apply PDenSetOrder_U. by apply ch.
+Qed.
+
+Definition Uapply_chain 
+    {qs : QvarScope} (qv : qs) (U : UnitaryOpt qv) (ch : chain qs) :=
+    mk_chain (Uapply_chain_prop U ch).
+
+(** We still need the assumption that addition is continuous *)
+Axiom unitary_continuous : 
+    forall {qs : QvarScope} (qv : qs) (U : UnitaryOpt qv) (ch : chain qs),
+    Uapply U (lim→∞ (ch)) = lim→∞ (Uapply_chain U ch).
+
+
+(* The chain of Mapply M ch result *)
+Definition Mapply_chain_obj 
+    {qs : QvarScope} (qv : qs) (M : MeaOpt qv) (ch : chain qs) (r : bool) :=
+    fun i => Mapply M (ch _[i]) r.
+Lemma Mapply_chain_prop 
+    {qs : QvarScope} (qv : qs) (M : MeaOpt qv) (ch : chain qs) (r : bool)
+    : forall i, Mapply_chain_obj M ch r i ⊑ Mapply_chain_obj M ch r i.+1.
+Proof.
+    rewrite /Mapply_chain_obj => i. apply PDenSetOrder_M. by apply ch.
+Qed.
+
+Definition Mapply_chain 
+    {qs : QvarScope} (qv : qs) (M : MeaOpt qv) (ch : chain qs) (r : bool) :=
+    mk_chain (Mapply_chain_prop M ch r).
+
+(** We still need the assumption that addition is continuous *)
+Axiom mea_continuous : forall {qs : QvarScope} 
+    (qv : qs) (M : MeaOpt qv) (ch : chain qs) (r : bool),
+    Mapply M (lim→∞ (ch)) r = lim→∞ (Mapply_chain M ch r).
+
+
+(* The chain of OpSemN ch (different from chain_OpSemN) *)
+Definition OpSemN_chain_obj {qs : QvarScope} (S : prog qs) (ch : chain qs) n :=
+    fun i => OpSemN <{S, ch _[i]}> n.
+
+Lemma OpSemN_chain_prop {qs : QvarScope} (S : prog qs) (ch : chain qs) n
+    : forall i, OpSemN_chain_obj S ch n i ⊑ OpSemN_chain_obj S ch n i.+1.
+Proof. 
+    rewrite /OpSemN_chain_obj => i. apply PDenSetOrder_OpSemN.
+    by apply ch.
+Qed.
+
+Definition OpSemN_chain {qs : QvarScope} (S : prog qs) (ch : chain qs) n :=
+    mk_chain (OpSemN_chain_prop S ch n).
+
+
+
+Theorem OpSemN_continuous (qs : QvarScope) (S : prog qs) (ch : chain qs) n:
+        OpSemN <{S, lim→∞ (ch)}> n = lim→∞ (OpSemN_chain S ch n).
+Proof.
+    elim: n S ch.
+    (* induction basis *)
+    move => S ch //=. apply PDenSetOrder_asymm.
+    by apply PDenSet_uni_least.
+    apply chain_limit_lub. rewrite /OpSemN_chain /OpSemN_chain_obj //=. by reflexivity.
+
+    (* induction step, case on program [S] *)
+    move => n IHn. case.
+    (* skip *)
+    move => ch.
+    rewrite /OpSemN_chain /OpSemN_chain_obj => //=. f_equal. 
+    by apply /chain_eqP.
+    (* abort *) 
+    move => ch //=. apply PDenSetOrder_asymm. 
+    by apply PDenSet_uni_least.
+    apply chain_limit_lub. rewrite /OpSemN_chain /OpSemN_chain_obj //=. 
+    by reflexivity.
+    (* init *)
+    move => ch qv //=. rewrite init_continuous. f_equal. 
+    apply /chain_eqP => //.
+    (* unitary *)
+    move => ch qv U //=. rewrite unitary_continuous. f_equal. 
+    apply /chain_eqP => //.
+    (* if *)
+    move => qv_m m S0 S1 ch. rewrite OpSemN_if.
+    rewrite !mea_continuous !IHn add_continuous. f_equal. apply /chain_eqP => //.
+    (* While *)
+    move => qv_m m S0 ch. rewrite OpSemN_while.
+    rewrite !mea_continuous IHn add_continuous. f_equal. apply /chain_eqP => //.
+    (* Seq *)
+    move => S1 S2 ch. rewrite OpSemN_seq.
+    rewrite !IHn. f_equal. apply /chain_eqP => //.
+    (* atom *)
+    move => S0 ch. rewrite OpSemN_atom.
+    rewrite IHn. f_equal. apply /chain_eqP => //.
+    (* parallel *)
+    move => S1 S2 ch. rewrite OpSemN_parallel.
+    rewrite !IHn union_continuous. f_equal. apply /chain_eqP => //.
+Qed.
+
+
+
+Lemma OpSem_seq {qs : QvarScope} S1 S2 (rho_s : PDenSet qs):
+    ⟦ S1 ;; S2 ⟧ (rho_s) =  ⟦ S2 ⟧ ( ⟦ S1 ⟧ (rho_s) ).
+Proof.
+    apply PDenSetOrder_asymm.
+
+    apply OpSem_lub. case. by apply PDenSet_uni_least.
+    move => n //=. transitivity (OpSemN <{ S2, ⟦ S1 ⟧ (rho_s) }> n).
+    apply PDenSetOrder_OpSemN. by apply OpSem_ub.
+    by apply OpSem_ub.
+
+    apply OpSem_lub => n.
+    rewrite [⟦ S1 ⟧(_)]/OpSem. rewrite OpSemN_continuous.
+    apply chain_limit_lub => i.
+    rewrite /OpSemN_chain /OpSemN_chain_obj //=.
+    
+    (* using [max i n] steps in [S1 ;; S2] *)
+    move : (OpSem_ub (max i n).+1 (S1;;S2) rho_s) => //=.
+    case E : (i <= n). 
+    { move /leP : E => E. rewrite (max_r _ _ E) => H.
+    transitivity (OpSemN <{ S2, OpSemN <{ S1, rho_s }> n }> n).
+    apply PDenSetOrder_OpSemN.
+    by apply /OpSemN_inc /leP.
+    by apply H. }
+    move /leP /Nat.lt_nge /Nat.lt_le_incl: E => E. rewrite (max_l _ _ E) => H.
+    transitivity (OpSemN <{ S2, OpSemN <{ S1, rho_s }> i }> i).
+    by apply /OpSemN_inc /leP.
+    by apply H.
+Qed.    
+
+Lemma OpSem_atom {qs : QvarScope} P (rho_s : PDenSet qs):
+    ⟦ <<P>> ⟧ (rho_s) =  ⟦ P ⟧ (rho_s).
+Proof.
+
+    apply PDenSetOrder_asymm.
+
+    apply OpSem_lub. case => //=. by apply PDenSet_uni_least.
+    move => n. by apply (OpSem_ub n).
+
+    apply OpSem_lub => n. rewrite -OpSemN_atom. by apply OpSem_ub.
+Qed.
+
+Lemma OpSem_para {qs : QvarScope} S1 S2 (rho_s : PDenSet qs):
+    ⟦ [S1 // S2] ⟧ (rho_s) = 
+        ⟦ Step S1 S2 true ⟧ (rho_s) ∪ ⟦ Step S1 S2 false ⟧ (rho_s).
+Proof.
+    apply PDenSetOrder_asymm.
+
+    apply OpSem_lub. case. by apply PDenSet_uni_least.
+    move => n. rewrite OpSemN_parallel. 
+    apply PDenSetOrder_union_split; by apply OpSem_ub.
+
+    rewrite ![⟦ Step _ _ _ ⟧(rho_s)]/OpSem. 
+    rewrite union_continuous. apply chain_limit_lub => l.
+    rewrite /chain_union /chain_union_obj /chain_OpSemN /chain_obj => //.
+    rewrite -OpSemN_parallel. by apply OpSem_ub.
+Qed.
+
 
     
 
-Lemma composition {qs : QvarScope} :
-    forall (rho_s : PDenSet qs) (S1 S2 : prog qs),
-        OpSem 
+
+
+
+    
